restruct code

code/hash/Hacl.Impl.SHA2.Core.fst
@@ -15,8 +15,8 @@ open Hacl.Hash.Definitions
 module Constants = Spec.SHA2.Constants
 module Spec = Spec.SHA2
 friend Hacl.Spec.SHA2.Vec
+module SpecVec = Hacl.Spec.SHA2.Vec
 open Hacl.Spec.SHA2.Vec
-
 #reset-options "--max_fuel 0 --max_ifuel 0 --z3rlimit 50"
 
 (** Top-level constant arrays for the SHA2 algorithms. *)
@@ -71,45 +71,9 @@ unfold let block_t (a:sha2_alg) =
 inline_for_extraction let multiblock (a:sha2_alg) (m:m_spec) =
    multibuf (lanes a m) (block_len a)
 
-let as_seq_multi (#lanes:lanes_t) (#len:size_t)
-                 (h:mem) (b:multibuf lanes len)
-                 : GTot (multiseq lanes (v len)) =
-    match lanes with
-    | 1 -> (as_seq h (b <: lbuffer uint8 len)) <: multiseq 1 (v len)
-    | 4 -> let (b0,(b1,(b2,b3))) = tup4 b in
-           let s0 = as_seq h (b0 <: lbuffer uint8 len) in
-           let s1 = as_seq h (b1 <: lbuffer uint8 len) in
-           let s2 = as_seq h (b2 <: lbuffer uint8 len) in
-           let s3 = as_seq h (b3 <: lbuffer uint8 len)  in
-           let ms : multiseq 4 (v len) = (s0,(s1,(s2,s3))) in
-           ms <: multiseq 4 (v len)
-    | _ -> admit()
-
-#push-options "--max_ifuel 4 --max_fuel 4"
-let as_seq_multi_lemma #lanes #len h b:
-  Lemma (forall i. i < lanes ==> (as_seq_multi #lanes #len h b).(|i|) == as_seq h b.(|i|))
-        [SMTPat (as_seq_multi #lanes #len h b)] =
-   match lanes with
-   | 1 -> ()
-   | 4 -> assert (lanes == 4);
-          let (b0,(b1,(b2,b3))) = tup4 b in
-          assert (b0 == b.(|0|));
-          assert (b1 == b.(|1|));
-          assert (b2 == b.(|2|));
-          assert (b3 == b.(|3|))
-   | _ -> admit()
-#pop-options
-
 inline_for_extraction
 let ws_t (a:sha2_alg) (m:m_spec) =
   lbuffer (element_t a m) 16ul
-
-noextract
-let ws_v (#a:sha2_alg) (#m:m_spec) (h:mem) (st:ws_t a m) : GTot (lseq (lseq (word a) 16) (lanes a m)) =
-  let st_seq = as_seq h st in
-  let st_seq_seq = Lib.Sequence.map vec_v st_seq in
-  let res = createi #(lseq (word a) 16) (lanes a m) (fun i -> map (fun x -> x.[i]) st_seq_seq) in
-  res
 
 inline_for_extraction
 val shuffle_core: #a: sha2_alg -> #m:m_spec ->
@@ -121,9 +85,9 @@ val shuffle_core: #a: sha2_alg -> #m:m_spec ->
     (ensures (fun h0 _ h1 ->
       modifies (loc st) h0 h1 /\
       as_seq h1 st ==
-      shuffle_core_spec k_t ws_t (as_seq h0 st)))
+      SpecVec.shuffle_core_spec k_t ws_t (as_seq h0 st)))
 
-#push-options "--z3rlimit 400 --max_fuel 2 --max_ifuel 2"
+#push-options "--z3rlimit 400"
 let shuffle_core #a #m k_t ws_t st =
   let hp0 = ST.get() in
   let a0 = st.(0ul) in
@@ -159,89 +123,166 @@ let shuffle_core #a #m k_t ws_t st =
 #pop-options
 
 inline_for_extraction
-val load_ws1 (#a: sha2_alg) (#m:m_spec{lanes a m = 1})
-             (b: block_t a) (ws: ws_t a m):
-    Stack unit
-    (requires (fun h ->
-      live h b /\ live h ws /\ disjoint b ws))
-    (ensures (fun h0 _ h1 ->
-      modifies (loc ws) h0 h1 /\
-      (let s0 : lseq uint8 (block_length a) = as_seq h0 b  in
-       let s0 : multiblock_spec a m = s0 <: multiseq 1 (block_length a) in
-       as_seq h1 ws == load_ws #a #m s0)))
-
-let load_ws1 #a #m b ws =
-    let h0 = ST.get() in
-    admit();
-    loop_nospec #h0 16ul ws (fun i ->
-      ws.(i) <- Lib.IntVector.vec_load_be (word_t a) 1 (sub b (i *. word_len a) (word_len a)))
+val set_wsi (#a:sha2_alg) (#m:m_spec) (ws:ws_t a m) (i:size_t{v i < 16}) (b:lbuffer uint8 (block_len a)) (bi:size_t{v bi < 16 / (lanes a m)}):
+            Stack unit
+            (requires (fun h -> live h b /\ live h ws /\ disjoint b ws))
+            (ensures (fun h0 _ h1 -> modifies (loc ws) h0 h1))
+let set_wsi #a #m ws i b bi =
+  [@inline_let]
+  let l = lanes a m in
+  ws.(i) <- vec_load_be (word_t a) l (sub b (bi *. size l *. word_len a) (size l *. word_len a))
 
 inline_for_extraction
-val load_ws4 (#a: sha2_alg) (#m:m_spec{lanes a m = 4})
-             (b: multiblock a m) (ws: ws_t a m):
+val load_blocks1 (#a: sha2_alg) (#m:m_spec{lanes a m == 1})
+                (b: multiblock a m) (ws: ws_t a m):
+    Stack unit
+    (requires (fun h -> live_multi h b /\ live h ws /\ disjoint_multi b ws))
+    (ensures (fun h0 _ h1 -> modifies (loc ws) h0 h1 /\
+                           as_seq h1 ws ==
+                           SpecVec.load_blocks (as_seq_multi h0 b)))
+let load_blocks1 #a #m b ws =
+  let h0 = ST.get() in
+  let b:lbuffer uint8 (block_len a) = b in
+  set_wsi ws 0ul b 0ul;
+  set_wsi ws 1ul b 1ul;
+  set_wsi ws 2ul b 2ul;
+  set_wsi ws 3ul b 3ul;
+  set_wsi ws 4ul b 4ul;
+  set_wsi ws 5ul b 5ul;
+  set_wsi ws 6ul b 6ul;
+  set_wsi ws 7ul b 7ul;
+  set_wsi ws 8ul b 8ul;
+  set_wsi ws 9ul b 9ul;
+  set_wsi ws 10ul b 10ul;
+  set_wsi ws 11ul b 11ul;
+  set_wsi ws 12ul b 12ul;
+  set_wsi ws 13ul b 13ul;
+  set_wsi ws 14ul b 14ul;
+  set_wsi ws 15ul b 15ul;
+  admit()
+
+inline_for_extraction
+val load_blocks4 (#a: sha2_alg) (#m:m_spec{lanes a m == 4})
+                 (b: multiblock a m) (ws: ws_t a m):
+    Stack unit
+    (requires (fun h -> live_multi h b /\ live h ws /\ disjoint_multi b ws))
+    (ensures (fun h0 _ h1 -> modifies (loc ws) h0 h1 /\
+                           as_seq h1 ws ==
+                           SpecVec.load_blocks (as_seq_multi h0 b)))
+
+#push-options "--max_fuel 4"
+let load_blocks4 #a #m b ws =
+  let h0 = ST.get() in
+  let (b0,(b1,(b2,b3))) = tup4 b in
+  set_wsi ws 0ul b0 0ul;
+  set_wsi ws 1ul b1 0ul;
+  set_wsi ws 2ul b2 0ul;
+  set_wsi ws 3ul b3 0ul;
+  set_wsi ws 4ul b0 1ul;
+  set_wsi ws 5ul b1 1ul;
+  set_wsi ws 6ul b2 1ul;
+  set_wsi ws 7ul b3 1ul;
+  set_wsi ws 8ul b0 2ul;
+  set_wsi ws 9ul b1 2ul;
+  set_wsi ws 10ul b2 2ul;
+  set_wsi ws 11ul b3 2ul;
+  set_wsi ws 12ul b0 3ul;
+  set_wsi ws 13ul b1 3ul;
+  set_wsi ws 14ul b2 3ul;
+  set_wsi ws 15ul b3 3ul;
+  admit()
+#pop-options
+
+inline_for_extraction
+val load_blocks (#a: sha2_alg) (#m:m_spec)
+                (b: multiblock a m) (ws: ws_t a m):
+    Stack unit
+    (requires (fun h -> live_multi h b /\ live h ws /\ disjoint_multi b ws))
+    (ensures (fun h0 _ h1 -> modifies (loc ws) h0 h1 /\
+                           as_seq h1 ws ==
+                           SpecVec.load_blocks (as_seq_multi h0 b)))
+
+let load_blocks #a #m b ws =
+  match lanes a m with
+  | 1 -> load_blocks1 b ws
+  | 4 -> load_blocks4 b ws
+  | _ -> admit()
+
+
+inline_for_extraction
+val transpose_ws4 (#a: sha2_alg) (#m:m_spec{lanes a m == 4}) (ws: ws_t a m):
+    Stack unit
+    (requires (fun h -> live h ws))
+    (ensures (fun h0 _ h1 -> modifies (loc ws) h0 h1 /\
+                           as_seq h1 ws ==
+                           SpecVec.transpose_ws (as_seq h0 ws)))
+
+let transpose_ws4 #a #m ws =
+  let (ws0,ws1,ws2,ws3) = transpose4x4 (ws.(0ul),ws.(1ul),ws.(2ul),ws.(3ul)) in
+  let (ws4,ws5,ws6,ws7) = transpose4x4 (ws.(4ul),ws.(5ul),ws.(6ul),ws.(7ul)) in
+  let (ws8,ws9,ws10,ws11) = transpose4x4 (ws.(8ul),ws.(9ul),ws.(10ul),ws.(11ul)) in
+  let (ws12,ws13,ws14,ws15) = transpose4x4 (ws.(12ul),ws.(13ul),ws.(14ul),ws.(15ul)) in
+  ws.(0ul) <- ws0;
+  ws.(1ul) <- ws1;
+  ws.(2ul) <- ws2;
+  ws.(3ul) <- ws3;
+  ws.(4ul) <- ws4;
+  ws.(5ul) <- ws5;
+  ws.(6ul) <- ws6;
+  ws.(7ul) <- ws7;
+  ws.(8ul) <- ws8;
+  ws.(9ul) <- ws9;
+  ws.(10ul) <- ws10;
+  ws.(11ul) <- ws11;
+  ws.(12ul) <- ws12;
+  ws.(13ul) <- ws13;
+  ws.(14ul) <- ws14;
+  ws.(15ul) <- ws15;
+  admit()
+
+inline_for_extraction
+val transpose_ws (#a: sha2_alg) (#m:m_spec) (ws: ws_t a m):
+    Stack unit
+    (requires (fun h -> live h ws))
+    (ensures (fun h0 _ h1 -> modifies (loc ws) h0 h1 /\
+                           as_seq h1 ws ==
+                           SpecVec.transpose_ws (as_seq h0 ws)))
+let transpose_ws #a #m ws =
+  match lanes a m with
+  | 1 -> ()
+  | 4 -> transpose_ws4 ws
+  | _ -> admit()
+
+
+inline_for_extraction
+val load_ws (#a: sha2_alg) (#m:m_spec)
+            (b: multiblock a m) (ws: ws_t a m):
     Stack unit
     (requires (fun h ->
       live_multi h b /\ live h ws /\ disjoint_multi b ws))
     (ensures (fun h0 _ h1 ->
       modifies (loc ws) h0 h1 /\
-      as_seq h1 ws == load_ws #a #m (as_seq_multi h0 b)
-      ))
-let load_ws4 #a #m b ws =
-    let (b0,(b1,(b2,b3))) = tup4 b in
-    admit();
-    let h0 = ST.get() in
-    loop_nospec #h0 4ul ws (fun i ->
-      ws.(4ul *. i) <- Lib.IntVector.vec_load_be (word_t a) 4 (sub b0 (4ul *. i *. word_len a) (4ul *. word_len a)));
-    let h0 = ST.get() in
-    loop_nospec #h0 4ul ws (fun i ->
-      ws.(4ul *. i +. 1ul) <- Lib.IntVector.vec_load_be (word_t a) 4 (sub b1 (4ul *. i *. word_len a) (4ul *. word_len a)));
-    let h0 = ST.get() in
-    loop_nospec #h0 4ul ws (fun i ->
-      ws.(4ul *. i +. 2ul) <- Lib.IntVector.vec_load_be (word_t a) 4 (sub b2 (4ul *. i *. word_len a) (4ul *. word_len a)));
-    let h0 = ST.get() in
-    loop_nospec #h0 4ul ws (fun i ->
-      ws.(4ul *. i +. 3ul) <- Lib.IntVector.vec_load_be (word_t a) 4 (sub b3 (4ul *. i *. word_len a) (4ul *. word_len a)));
-    let h0 = ST.get() in
-    loop_nospec #h0 4ul ws (fun i ->
-      let ws0 = ws.(4ul*.i+.0ul) in
-      let ws1 = ws.(4ul*.i+.1ul) in
-      let ws2 = ws.(4ul*.i+.2ul) in
-      let ws3 = ws.(4ul*.i+.3ul) in
-      let (ws0,ws1,ws2,ws3) = transpose4x4 (ws0,ws1,ws2,ws3) in
-      ws.(4ul*.i) <- ws0;
-      ws.(4ul*.i+.1ul) <- ws1;
-      ws.(4ul*.i+.2ul) <- ws2;
-      ws.(4ul*.i+.3ul) <- ws3)
-
-#push-options "--max_ifuel 2 --max_fuel 2 --z3rlimit 100"
-inline_for_extraction
-val load_ws (#a: sha2_alg) (#m:m_spec)
-            (b: multiblock a m) (ws: ws_t a m):
-    Stack unit
-    (requires (fun h -> live_multi h b /\ live h ws /\ disjoint_multi b ws))
-    (ensures (fun h0 _ h1 -> modifies (loc ws) h0 h1 /\
-                           as_seq h1 ws == load_ws (as_seq_multi h0 b)))
+      as_seq h1 ws == SpecVec.load_ws #a #m (as_seq_multi h0 b)))
 let load_ws #a #m b ws =
-  match lanes a m with
-  | 1 -> load_ws1 b ws
-  | 4 -> load_ws4 b ws
-  | _ -> admit()
-#pop-options
+    let h0 = ST.get() in
+    load_blocks b ws;
+    transpose_ws ws
 
+#push-options "--z3rlimit 200"
 inline_for_extraction
 val ws_next (#a: sha2_alg) (#m:m_spec)
-            (k:size_t{size_v k > 0 /\ size_v k < size_v (num_rounds16 a)}) (ws: ws_t a m):
+            (ws: ws_t a m):
     Stack unit
     (requires (fun h -> live h ws))
     (ensures (fun h0 _ h1 ->
       modifies (loc ws) h0 h1 /\
-      as_seq h1 ws == ws_next (v k) (as_seq h0 ws)))
-let ws_next #a #m k ws =
+      as_seq h1 ws == SpecVec.ws_next (as_seq h0 ws)))
+let ws_next #a #m ws =
   let h0 = ST.get() in
   loop1 h0 16ul ws
-    (fun h -> ws_next_inner #a #m (v k))
+    (fun h -> ws_next_inner #a #m)
     (fun i ->
-      Lib.LoopCombinators.unfold_repeati 16 (ws_next_inner #a #m (v k)) (as_seq h0 ws) (v i);
+      Lib.LoopCombinators.unfold_repeati 16 (ws_next_inner #a #m) (as_seq h0 ws) (v i);
       let t16 = ws.(i) in
       let t15 = ws.((i+.1ul) %. 16ul) in
       let t7  = ws.((i+.9ul) %. 16ul) in
@@ -249,6 +290,7 @@ let ws_next #a #m k ws =
       let s1 = _sigma1 t2 in
       let s0 = _sigma0 t15 in
       ws.(i) <- (s1 +| t7 +| s0 +| t16))
+#pop-options
 
 inline_for_extraction
 val shuffle: #a:sha2_alg -> #m:m_spec -> ws:ws_t a m -> hash:state_t a m ->
@@ -258,7 +300,7 @@ val shuffle: #a:sha2_alg -> #m:m_spec -> ws:ws_t a m -> hash:state_t a m ->
       disjoint hash ws))
     (ensures (fun h0 _ h1 ->
       modifies2 ws hash h0 h1 /\
-      as_seq h1 hash == shuffle #a #m (as_seq h0 ws) (as_seq h0 hash)))
+      as_seq h1 hash == SpecVec.shuffle #a #m (as_seq h0 ws) (as_seq h0 hash)))
 
 let shuffle #a #m ws hash =
   let h0 = ST.get() in
@@ -275,7 +317,7 @@ let shuffle #a #m ws hash =
        let ws_t = ws.(j) in
        shuffle_core k_t ws_t hash);
       if i <. num_rounds16 a -. 1ul then
-        ws_next (i+.1ul) ws)
+        ws_next ws)
 
 
 (** Init *)
@@ -291,7 +333,7 @@ val init: #a:sha2_alg -> #m:m_spec -> hash:state_t a m ->
     Stack unit
     (requires (fun h -> live h hash))
     (ensures (fun h0 _ h1 -> modifies1 hash h0 h1 /\
-                           as_seq h1 hash == init #a #m))
+                           as_seq h1 hash == SpecVec.init a m))
 let init #a #m hash =
   let h0 = ST.get() in
   fill h0 8ul hash
@@ -304,14 +346,15 @@ let init #a #m hash =
 
 let update_t (a:sha2_alg) (m:m_spec) = b:multiblock a m -> hash:state_t a m ->
     Stack unit
-    (requires (fun h -> live_multi h b /\ live h hash /\ disjoint_multi b hash))
+    (requires (fun h -> live_multi h b /\ live h hash))// /\ disjoint_multi b hash))
     (ensures (fun h0 _ h1 -> modifies (loc hash) h0 h1 /\
-                           as_seq h1 hash == update (as_seq_multi h0 b) (as_seq h0 hash)))
+                           as_seq h1 hash == SpecVec.update (as_seq_multi h0 b) (as_seq h0 hash)))
 
-#push-options "--max_fuel 0 --max_ifuel 0 --z3rlimit 200"
+#push-options "--max_fuel 3 --max_ifuel 2 --z3rlimit 500"
 inline_for_extraction
 val update: #a:sha2_alg -> #m:m_spec -> update_t a m
 let update #a #m b hash =
+  let init_h0 = ST.get() in
   push_frame ();
   let h0 = ST.get() in
   let hash_old = create 8ul (zero_element a m) in
@@ -336,48 +379,118 @@ let update #a #m b hash =
   let h4 = ST.get() in
   assert (as_seq h4 hash_old == as_seq h1 hash_old);
   assert (as_seq h4 hash == Hacl.Spec.SHA2.Vec.shuffle (as_seq h3 ws) (as_seq h0 hash));
-  assert (modifies (loc ws |+| loc hash_old |+| loc hash) h0 h4);
+  assert (modifies (loc hash |+| (loc ws |+| loc hash_old)) h0 h4);
   map2T 8ul hash (+|) hash hash_old; 
   let h5 = ST.get() in
   assert (as_seq h5 hash == map2 (+|) (as_seq h4 hash) (as_seq h1 hash_old));
   assert (as_seq h5 hash == update (as_seq_multi h0 b) (as_seq h0 hash));
-  admit();
-  pop_frame()
+  assert (modifies (loc hash |+| (loc ws |+| loc hash_old)) h0 h5);
+  pop_frame();
+  let fin_h5 = ST.get() in
+  assert (modifies (loc hash) init_h0 fin_h5)
 #pop-options
 
 inline_for_extraction
 let padded_blocks (a:sha2_alg) (len:size_t{v len < block_length a}) =
   if (len +. len_len a +. 1ul <=. block_len a) then 1ul else 2ul
 
-inline_for_extraction
-val update1_last: #a:sha2_alg -> #m:m_spec{lanes a m = 1} ->
-                  upd: update_t a m ->
-                  totlen:len_t a ->
-                  len:size_t{v len < block_length a} ->
-                  b:lbuffer uint8 len -> hash:state_t a m ->
-    Stack unit
-    (requires (fun h -> live h b /\ live h hash /\ disjoint b hash))
-    (ensures (fun h0 _ h1 -> modifies1 hash h0 h1))
-let update1_last #a #m upd totlen len b hash =
-  push_frame ();
-  let last = create (2ul *. block_len a) (u8 0) in
-  copy (sub last 0ul len) b;
-  last.(len) <- u8 0x80;
-  let total_len_bits = secret (shift_left #(len_int_type a) totlen 3ul) in 
-  let blocks = padded_blocks a len in
-  let fin = blocks *. block_len a in
-  let len_by = sub last (fin -. len_len a) (len_len a) in
-  Lib.ByteBuffer.uint_to_bytes_be #(len_int_type a) len_by total_len_bits;
-  let b0 = sub last 0ul (block_len a) in
-  upd b0 hash;
-  if blocks >. 1ul then (
-    let b1 = sub last (block_len a) (block_len a) in
-    upd b1 hash
-  );
-  pop_frame()
 
 inline_for_extraction
-val update4_last: #a:sha2_alg -> #m:m_spec{lanes a m = 4} ->
+val load_last1: #a:sha2_alg -> #m:m_spec{lanes a m = 1} ->
+                  totlen_buf:lbuffer uint8 (len_len a) ->
+                  len:size_t{v len < block_length a} ->
+                  b:lbuffer uint8 len ->
+                  fin:size_t{v fin == block_length a \/ v fin == 2 * block_length a} ->
+                  last:lbuffer uint8 (2ul *. block_len a) ->
+    Stack (lbuffer uint8 (block_len a) & lbuffer uint8 (block_len a))
+    (requires (fun h -> live h totlen_buf /\ live h b /\ live h last /\
+                      disjoint last b /\ disjoint last totlen_buf /\
+                      as_seq h last == Lib.Sequence.create (2 * block_length a) (u8 0)))
+    (ensures (fun h0 (l0,l1) h1 -> modifies (loc last) h0 h1 /\
+                           live h1 l0 /\ live h1 l1 /\
+                           (as_seq h1 l0, as_seq h1 l1) ==
+                           load_last1 #a #m (as_seq h0 totlen_buf) (v fin) (v len) (as_seq h0 b)))
+let load_last1 #a #m totlen_buf len b fin last =
+  update_sub last 0ul len b;
+  last.(len) <- u8 0x80;
+  update_sub last (fin -. len_len a) (len_len a) totlen_buf;
+  let last0 = sub last 0ul (block_len a) in
+  let last1 = sub last (block_len a) (block_len a) in
+  (last0,last1)
+
+inline_for_extraction
+val load_last4: #a:sha2_alg -> #m:m_spec{lanes a m = 4} ->
+                  totlen_buf:lbuffer uint8 (len_len a) ->
+                  len:size_t{v len < block_length a} ->
+                  b:multibuf (lanes a m) len ->
+                  fin:size_t{v fin == block_length a \/ v fin == 2 * block_length a} ->
+                  last:lbuffer uint8 (size (lanes a m) *. 2ul *. block_len a) ->
+    Stack (multibuf (lanes a m) (block_len a) & multibuf (lanes a m) (block_len a))
+    (requires (fun h -> live h totlen_buf /\ live_multi h b /\ live h last /\
+                      disjoint_multi b last /\ disjoint last totlen_buf /\
+                      as_seq h last == Lib.Sequence.create (lanes a m * 2 * block_length a) (u8 0)))
+    (ensures (fun h0 (l0,l1) h1 -> modifies (loc last) h0 h1 /\
+                           live_multi h1 l0 /\ live_multi h1 l1 /\
+                           (as_seq_multi h1 l0, as_seq_multi h1 l1) ==
+                           load_last4 #a #m (as_seq h0 totlen_buf) (v fin) (v len) (as_seq_multi h0 b)))
+
+#push-options "--max_ifuel 4 --max_fuel 4 --z3rlimit 300"
+let load_last4 #a #m totlen_buf len b fin last =
+  let (b0,(b1,(b2,b3))) = tup4 b in
+  let last0 = sub last 0ul (2ul *. block_len a) in
+  let last1 = sub last (2ul *. block_len a) (2ul *. block_len a) in
+  let last2 = sub last (4ul *. block_len a) (2ul *. block_len a) in
+  let last3 = sub last (6ul *. block_len a) (2ul *. block_len a) in
+  admit();
+  update_sub last0 0ul len b0;
+  update_sub last1 0ul len b1;
+  update_sub last2 0ul len b2;
+  update_sub last3 0ul len b3;
+  last0.(len) <- u8 0x80;
+  last1.(len) <- u8 0x80;
+  last2.(len) <- u8 0x80;
+  last3.(len) <- u8 0x80;
+  update_sub last0 (fin -. len_len a) (len_len a) totlen_buf;
+  update_sub last1 (fin -. len_len a) (len_len a) totlen_buf;
+  update_sub last2 (fin -. len_len a) (len_len a) totlen_buf;
+  update_sub last3 (fin -. len_len a) (len_len a) totlen_buf;
+  let l00 = sub last0 0ul (block_len a) in
+  let l10 = sub last1 0ul (block_len a) in
+  let l20 = sub last2 0ul (block_len a) in
+  let l30 = sub last3 0ul (block_len a) in
+  let l01 = sub last0 (block_len a) (block_len a) in
+  let l11 = sub last1 (block_len a) (block_len a) in
+  let l21 = sub last2 (block_len a) (block_len a) in
+  let l31 = sub last3 (block_len a) (block_len a) in
+  let mb0:multibuf 4 (block_len a) = (l00, (l10, (l20, l30))) in
+  let mb1:multibuf 4 (block_len a) = (l01, (l11, (l21, l31))) in
+  (mb0, mb1)  
+#pop-options
+
+inline_for_extraction
+val load_last: #a:sha2_alg -> #m:m_spec ->
+               totlen_buf:lbuffer uint8 (len_len a) ->
+               len:size_t{v len < block_length a} ->
+               b:multibuf (lanes a m) len ->
+               fin:size_t{v fin == block_length a \/ v fin == 2 * block_length a} ->
+               last:lbuffer uint8 (size (lanes a m) *. 2ul *. block_len a) ->
+    Stack (multibuf (lanes a m) (block_len a) & multibuf (lanes a m) (block_len a))
+    (requires (fun h -> live h totlen_buf /\ live_multi h b /\ live h last /\
+                      disjoint_multi b last /\ disjoint last totlen_buf /\
+                      as_seq h last == Lib.Sequence.create (lanes a m * 2 * block_length a) (u8 0)))
+    (ensures (fun h0 (l0,l1) h1 -> modifies (loc last) h0 h1 /\
+                           live_multi h1 l0 /\ live_multi h1 l1 /\
+                           (as_seq_multi h1 l0, as_seq_multi h1 l1) ==
+                           SpecVec.load_last #a #m (as_seq h0 totlen_buf) (v fin) (v len) (as_seq_multi h0 b)))
+
+let load_last #a #m  totlen_buf len b fin last =
+  match lanes a m with
+  | 1 -> load_last1 #a #m totlen_buf len b fin last
+  | 4 -> load_last4 #a #m totlen_buf len b fin last
+  | _ -> admit()
+  
+inline_for_extraction
+val update_last: #a:sha2_alg -> #m:m_spec ->
                   upd: update_t a m ->
                   totlen:len_t a ->
                   len:size_t{v len < block_length a} ->
@@ -385,123 +498,119 @@ val update4_last: #a:sha2_alg -> #m:m_spec{lanes a m = 4} ->
                   hash:state_t a m ->
     Stack unit
     (requires (fun h -> live_multi h b /\ live h hash /\ disjoint_multi b hash))
-    (ensures (fun h0 _ h1 -> modifies1 hash h0 h1))
+    (ensures (fun h0 _ h1 -> modifies (loc hash) h0 h1))
+
 #push-options "--z3rlimit 200"
-let update4_last #a #m upd totlen len b hash =
+let update_last #a #m upd totlen len b hash =
   push_frame ();
-  let (b0,(b1,(b2,b3))) = tup4 b in
-  admit();
-  let last = create (8ul *. block_len a) (u8 0) in
-  let last0 = sub last 0ul (2ul *. block_len a) in
-  let last1 = sub last (2ul *. block_len a) (2ul *. block_len a) in
-  let last2 = sub last (4ul *. block_len a) (2ul *. block_len a) in
-  let last3 = sub last (6ul *. block_len a) (2ul *. block_len a) in
-  copy (sub last0 0ul len) b0;
-  copy (sub last1 0ul len) b1;
-  copy (sub last2 0ul len) b2;
-  copy (sub last3 0ul len) b3;
-  last0.(len) <- u8 0x80;
-  last1.(len) <- u8 0x80;
-  last2.(len) <- u8 0x80;
-  last3.(len) <- u8 0x80;
+  let last = create (size (lanes a m) *. 2ul *. block_len a) (u8 0) in
+  let totlen_buf = create (len_len a) (u8 0) in
   let total_len_bits = secret (shift_left #(len_int_type a) totlen 3ul) in 
+  Lib.ByteBuffer.uint_to_bytes_be #(len_int_type a) totlen_buf total_len_bits;
   let blocks = padded_blocks a len in
   let fin = blocks *. block_len a in
-  let len_buf0 = sub last0 (fin -. len_len a) (len_len a) in
-  let len_buf1 = sub last1 (fin -. len_len a) (len_len a) in
-  let len_buf2 = sub last2 (fin -. len_len a) (len_len a) in
-  let len_buf3 = sub last3 (fin -. len_len a) (len_len a) in
-  Lib.ByteBuffer.uint_to_bytes_be #(len_int_type a) len_buf0 total_len_bits;
-  Lib.ByteBuffer.uint_to_bytes_be #(len_int_type a) len_buf1 total_len_bits;
-  Lib.ByteBuffer.uint_to_bytes_be #(len_int_type a) len_buf2 total_len_bits;
-  Lib.ByteBuffer.uint_to_bytes_be #(len_int_type a) len_buf3 total_len_bits;
-  let last00 = sub last0 0ul (block_len a) in
-  let last10 = sub last1 0ul (block_len a) in
-  let last20 = sub last2 0ul (block_len a) in
-  let last30 = sub last3 0ul (block_len a) in
-  let mb:multibuf 4 (block_len a) = (last00, (last10, (last20, last30))) in
-  upd mb hash;
+  let (last0,last1) = load_last #a #m totlen_buf len b fin last in
+  upd last0 hash;
   if blocks >. 1ul then (
-    let last01 = sub last0 (block_len a) (block_len a) in
-    let last11 = sub last1 (block_len a) (block_len a) in
-    let last21 = sub last2 (block_len a) (block_len a) in
-    let last31 = sub last3 (block_len a) (block_len a) in
-    let mb: multibuf 4 (block_len a) = (last01, (last11, (last21, last31))) in
-    upd mb hash
+    upd last1 hash
   );
   pop_frame()
 #pop-options
 
 inline_for_extraction
-val update_last: #a:sha2_alg -> #m:m_spec ->
-                  upd: update_t a m ->
-                  totlen:len_t a ->
-                  len:size_t{v len < block_length a} ->
-                  b:multibuf (lanes a m) len -> hash:state_t a m ->
+val transpose_state4 (#a: sha2_alg) (#m:m_spec{lanes a m == 4}) (st: state_t a m):
     Stack unit
-    (requires (fun h -> live_multi h b /\ live h hash /\ disjoint_multi b hash))
-    (ensures (fun h0 _ h1 -> modifies1 hash h0 h1))
+    (requires (fun h -> live h st))
+    (ensures (fun h0 _ h1 -> modifies (loc st) h0 h1 /\
+                           as_seq h1 st ==
+                           SpecVec.transpose_hash4 (as_seq h0 st)))
 
-let update_last #a #m upd totlen len b hash =
+let transpose_state4 #a #m st =
+  let (st0,st1,st2,st3) = transpose4x4 (st.(0ul),st.(1ul),st.(2ul),st.(3ul)) in
+  let (st4,st5,st6,st7) = transpose4x4 (st.(4ul),st.(5ul),st.(6ul),st.(7ul)) in
+  st.(0ul) <- st0;
+  st.(1ul) <- st4;
+  st.(2ul) <- st1;
+  st.(3ul) <- st5;
+  st.(4ul) <- st2;
+  st.(5ul) <- st6;
+  st.(6ul) <- st3;
+  st.(7ul) <- st7;
+  admit()
+
+inline_for_extraction
+val transpose_state (#a: sha2_alg) (#m:m_spec) (st: state_t a m):
+    Stack unit
+    (requires (fun h -> live h st))
+    (ensures (fun h0 _ h1 -> modifies (loc st) h0 h1 /\
+                           as_seq h1 st ==
+                           SpecVec.transpose_hash (as_seq h0 st)))
+let transpose_state #a #m st =
   match lanes a m with
-  | 1 -> update1_last upd totlen len b hash
-  | 4 -> update4_last upd totlen len b hash
+  | 1 -> ()
+  | 4 -> transpose_state4 st
   | _ -> admit()
 
 
 inline_for_extraction
-val finish1: #a:sha2_alg -> #m:m_spec{lanes a m = 1} ->
-             b:lbuffer uint8 (hash_len a) -> hash:state_t a m ->
+val store_state: #a:sha2_alg -> #m:m_spec->
+                 st:state_t a m ->
+                 hbuf:lbuffer uint8 (size (lanes a m) *. 8ul *. word_len a) ->
     Stack unit
-    (requires (fun h -> live h b /\ live h hash /\ disjoint b hash))
-    (ensures (fun h0 _ h1 -> modifies1 b h0 h1))
-let finish1 #a #m b hash =
+    (requires (fun h -> live h hbuf /\ live h st /\ disjoint hbuf st))
+    (ensures (fun h0 _ h1 -> modifies (loc st |+| loc hbuf) h0 h1))
+let store_state #a #m st hbuf =
+  transpose_state st;
   let h0 = ST.get() in
-  loop_nospec #h0 (hash_word_len a) b (fun i ->
-       vec_store_be (sub b (i *. word_len a) (word_len a)) hash.(i))
+  [@inline_let]
+  let spec_inner st0 (i:size_nat{i < 8}) (hseq:lseq uint8 (lanes a m * 8 * word_length a)) =
+    Lib.Sequence.update_sub hseq (i * lanes a m * word_length a) (lanes a m * word_length a)
+                                          (vec_to_bytes_be st0.[i]) in
+  loop1 h0 8ul hbuf
+  (fun h -> spec_inner (as_seq h0 st))
+  (fun i ->  
+    admit();
+    Lib.LoopCombinators.unfold_repeati 8 (spec_inner (as_seq h0 st)) (as_seq h0 hbuf) (v i);
+    vec_store_be (sub hbuf (size (lanes a m) *. i *. word_len a) (size (lanes a m) *. word_len a)) st.(i))
 
 inline_for_extraction
-val finish4: #a:sha2_alg -> #m:m_spec{lanes a m = 4} ->
-             b:multibuf (lanes a m) (hash_len a) ->
-             hash:state_t a m ->
+val emit1: #a:sha2_alg -> #m:m_spec{lanes a m = 1} ->
+             hbuf: lbuffer uint8 (8ul *. word_len a) ->
+             result:lbuffer uint8 (hash_len a) ->
     Stack unit
-    (requires (fun h -> live_multi h b /\ live h hash /\ disjoint_multi b hash))
-    (ensures (fun h0 _ h1 -> modifies_multi b h0 h1))
-let finish4 #a #m b hash =
-  push_frame();
-  let (b0,(b1,(b2,b3))) = tup4 b in
-  admit();
-  let hbuf = create (4ul *. 8ul *. word_len a) (u8 0) in 
-  let h0 = ST.get() in
-  loop_nospec #h0 8ul hbuf (fun i ->
-       vec_store_be (sub hbuf (4ul *. i *. word_len a) (4ul *. word_len a)) hash.(i));
-  let h0 = ST.get() in
-  loop_nospec #h0 (hash_word_len a) b0 (fun i ->
-       copy (sub b0 (i *. word_len a) (word_len a)) (sub hbuf (4ul*.i*.word_len a) (word_len a)));
-  let h0 = ST.get() in
-  loop_nospec #h0 (hash_word_len a) b1 (fun i ->
-       copy (sub b1 (i *. word_len a) (word_len a)) (sub hbuf (4ul*.i*.word_len a+.word_len a) (word_len a)));
-  let h0 = ST.get() in
-  loop_nospec #h0 (hash_word_len a) b2 (fun i ->
-       copy (sub b2 (i *. word_len a) (word_len a)) (sub hbuf (4ul*.i*.word_len a+.2ul*.word_len a) (word_len a)));
-  let h0 = ST.get() in
-  loop_nospec #h0 (hash_word_len a) b3 (fun i ->
-       copy (sub b3 (i *. word_len a) (word_len a)) (sub hbuf (4ul*.i*.word_len a+.3ul*.word_len a) (word_len a)));
-  pop_frame()
+    (requires (fun h -> live h result /\ live h hbuf /\ disjoint result hbuf))
+    (ensures (fun h0 _ h1 -> modifies (loc result) h0 h1))
+let emit1 #a #m hbuf result =
+  copy result (sub hbuf 0ul (hash_len a))
 
 inline_for_extraction
-val finish: #a:sha2_alg -> #m:m_spec ->
-             b:multibuf (lanes a m) (hash_len a) ->
-             hash:state_t a m ->
+val emit4: #a:sha2_alg -> #m:m_spec{lanes a m = 4} ->
+             hbuf: lbuffer uint8 (size (lanes a m) *. 8ul *. word_len a) ->
+             result:multibuf (lanes a m) (hash_len a) ->
     Stack unit
-    (requires (fun h -> live_multi h b /\ live h hash /\ disjoint_multi b hash))
-    (ensures (fun h0 _ h1 -> modifies_multi b h0 h1))
+    (requires (fun h -> live_multi h result /\ live h hbuf /\ disjoint_multi result hbuf))
+    (ensures (fun h0 _ h1 -> modifies_multi result h0 h1))
+#push-options "--max_fuel 4 --z3rlimit 200"
+let emit4 #a #m hbuf result =
+  let (b0,(b1,(b2,b3))) = tup4 result in
+  copy b0 (sub hbuf 0ul (hash_len a));
+  copy b1 (sub hbuf (8ul *. word_len a) (hash_len a));
+  copy b2 (sub hbuf (16ul *. word_len a) (hash_len a));
+  copy b3 (sub hbuf (24ul *. word_len a) (hash_len a))
+#pop-options
 
-#push-options "--z3rlimit 200"
-let finish #a #m b hash =
+
+inline_for_extraction
+val emit: #a:sha2_alg -> #m:m_spec ->
+          hbuf: lbuffer uint8 (size (lanes a m) *. 8ul *. word_len a) ->
+          result:multibuf (lanes a m) (hash_len a) ->
+    Stack unit
+    (requires (fun h -> live_multi h result /\ live h hbuf /\ disjoint_multi result hbuf))
+    (ensures (fun h0 _ h1 -> modifies_multi result h0 h1))
+let emit #a #m hbuf result =
   match lanes a m with
-  | 1 -> finish1 #a #m b hash
-  | 4 -> finish4 #a #m b hash
+  | 1 -> emit1 #a #m hbuf result
+  | 4 -> emit4 #a #m hbuf result
   | _ -> admit()
 
 inline_for_extraction
@@ -572,15 +681,17 @@ let hash #a #m upd h len b =
     let len' : len_t a = Lib.IntTypes.cast #U32 #PUB (len_int_type a) PUB len in
     admit();
     update_last #a #m upd len' rem mb st;
-    finish h st;
+    let hbuf = create (size (lanes a m) *. 8ul *. word_len a) (u8 0) in
+    store_state st hbuf;
+    emit hbuf h;
     pop_frame()
 
 [@CInline]
-val sha256_update1: b:block_t SHA2_256 -> hash:state_t SHA2_256 M32 ->
+val sha256_update1: b:multiblock SHA2_256 M32 -> hash:state_t SHA2_256 M32 ->
     Stack unit
-    (requires (fun h -> live h b /\ live h hash /\ disjoint b hash))
-    (ensures (fun h0 _ h1 -> modifies1 hash h0 h1 /\
-                           as_seq h1 hash == Hacl.Spec.SHA2.Vec.update #SHA2_256 #M32 (as_seq h0 b) (as_seq h0 hash)))
+    (requires (fun h -> live_multi h b /\ live h hash))// /\ disjoint_multi b hash))
+    (ensures (fun h0 _ h1 -> modifies (loc hash) h0 h1 /\
+                           as_seq h1 hash == Hacl.Spec.SHA2.Vec.update #SHA2_256 #M32 (as_seq_multi h0 b) (as_seq h0 hash)))
 let sha256_update1 b hash = update #SHA2_256 #M32 b hash
 
 let sha256 h len b = hash #SHA2_256 #M32 sha256_update1 h len (b <: lbuffer uint8 len)
@@ -589,7 +700,7 @@ let sha256 h len b = hash #SHA2_256 #M32 sha256_update1 h len (b <: lbuffer uint
 val sha256_update4: b:multiblock SHA2_256 M128 ->
                     hash:state_t SHA2_256 M128 ->
     Stack unit
-    (requires (fun h -> live_multi h b /\ live h hash /\ disjoint_multi b hash))
+    (requires (fun h -> live_multi h b /\ live h hash))// /\ disjoint_multi b hash))
     (ensures (fun h0 _ h1 -> modifies1 hash h0 h1 /\
                            as_seq h1 hash == Hacl.Spec.SHA2.Vec.update #SHA2_256 #M128 (as_seq_multi h0 b) (as_seq h0 hash)))
 
@@ -604,3 +715,5 @@ let sha256_4 r0 r1 r2 r3 len b0 b1 b2 b3 =
   assert (live_multi h0 ib);
   hash #SHA2_256 #M128 sha256_update4 rb len ib
 #pop-options
+
+
