code/hash/Lib.MultiBuffer.fst
@@ -35,6 +35,17 @@ let modifies_multi #lanes #len (b:multibuf lanes len) (h0:mem) (h1:mem) =
 let stack_allocated_multi #lanes #len (b:multibuf lanes len) (h0:mem) (h1:mem) (s:lseq uint8 (v len)) =
   forall i. i < lanes ==> stack_allocated b.(|i|) h0 h1 s
 
+let multiseq (lanes:flen) (len:size_nat) =
+    ntuple (lseq uint8 len) lanes
+let as_seq_multi #lanes #len (h:mem) (b:multibuf lanes len) : GTot (multiseq lanes (v len)) =
+    gmap (as_seq h) b
+
+let as_seq_multi_lemma #lanes #len h b:
+  Lemma (forall i. i < lanes ==> (as_seq_multi #lanes #len h b).(|i|) == as_seq h b.(|i|))
+        [SMTPat (as_seq_multi #lanes #len h b)] = ()
+  
+
+
 (*
 inline_for_extraction
 val sub_multi: #lanes:flen -> #len:size_t -> b:multibuf lanes len -> start:size_t -> slen:size_t{v start + v slen <= v len} -> Stack (multibuf lanes slen)
